sigma_glu_typ_pred was incorrect

theories/Core/Soundness/LogicalRelation/Definitions.v
@@ -106,20 +106,19 @@ Variant pi_glu_exp_pred i
 
 Variant sigma_glu_typ_pred i
   (FR : relation domain)
-  (IP : glu_typ_pred)
+  (FP : glu_typ_pred)
   (FEl : glu_exp_pred)
   (SP : forall c (equiv_c : {{ Dom c ≈ c ∈ FR }}), glu_typ_pred) : glu_typ_pred :=
 | mk_sigma_glu_typ_pred :
-  `{ {{ Γ ⊢ A ≈ Σ FT ST : Type@i }} ->
+  `{ forall (equiv_m : {{ Dom m ≈ m ∈ FR }}),
+     {{ Γ ⊢ A ≈ Σ FT ST : Type@i }} ->
      {{ Γ ⊢ FT : Type@i }} ->
      {{ Γ , FT ⊢ ST : Type@i }} ->
-     (forall Δ σ, {{ Δ ⊢w σ : Γ }} -> {{ Δ ⊢ IT[σ] ® IP }}) ->
-     (forall Δ σ M m,
-         {{ Δ ⊢w σ : Γ }} ->
-         {{ Δ ⊢ M : FT[σ] ® m ∈ FEl }} ->
-         forall (equiv_m : {{ Dom m ≈ m ∈ FR }}),
-           {{ Δ ⊢ OT[σ,,M] ® SP _ equiv_m }}) ->
-     {{ Γ ⊢ A ® sigma_glu_typ_pred i FR IP FEl SP }} }.
+     {{ Γ ⊢ M : FT }} ->
+     (forall Δ σ, {{ Δ ⊢w σ : Γ }} -> {{ Δ ⊢ FT[σ] ® FP }}) ->
+     (forall Δ σ, {{ Δ ⊢w σ : Γ }} ->
+         {{ Δ ⊢ M[σ] : FT[σ] ® m ∈ FEl }} /\ {{ Δ ⊢ ST[σ,,M[σ]] ® SP _ equiv_m }}) ->
+     {{ Γ ⊢ A ® sigma_glu_typ_pred i FR FP FEl SP }} }.
 
 Variant sigma_glu_exp_pred i
   (FR : relation domain)
@@ -129,18 +128,19 @@ Variant sigma_glu_exp_pred i
   (* should SEl be parameterized over equiv_c? *)
   (SEl : forall c (equiv_c : {{ Dom c ≈ c ∈ FR }}), glu_exp_pred): glu_exp_pred :=
 | mk_sigma_glu_exp_pred :
-  `{ {{ Γ ⊢ M : A }} ->
+  `{ forall (equiv_m : {{ Dom m1 ≈ m1 ∈ FR }}),
+     {{ Γ ⊢ M : A }} ->
      {{ Dom m ≈ m ∈ elem_rel }} ->
+     {{ π₁ m ↘ m1 }} -> 
+     {{ π₂ m ↘ m2 }} ->
      {{ Γ ⊢ A ≈ Σ FT ST : Type@i }} ->
      {{ Γ ⊢ FT : Type@i }} ->
      {{ Γ , FT ⊢ ST : Type@i }} ->
      (forall Δ σ, {{ Δ ⊢w σ : Γ }} -> {{ Δ ⊢ FT[σ] ® FP }}) ->
      (forall Δ σ,
-         {{ Δ ⊢w σ : Γ }} ->
-         exists m1 m2 (equiv_n : {{ Dom m1 ≈ m1 ∈ FR }}),
-          {{ π₁ m ↘ m1 }} /\ {{ π₂ m ↘ m2 }} /\ 
-          {{ Δ ⊢ fst M[σ] : FT[σ] ® m1 ∈ FEl }} /\
-          {{ Δ ⊢ snd M[σ] : ST[σ,,fst M[σ]] ® m2 ∈ SEl _ equiv_n }} ) ->
+         {{ Δ ⊢w σ : Γ }} ->          
+          {{ Δ ⊢ (fst M)[σ] : FT[σ] ® m1 ∈ FEl }} /\
+          {{ Δ ⊢ (snd M)[σ] : ST[σ,,(fst M)[σ]] ® m2 ∈ SEl _ equiv_m }} ) ->
      {{ Γ ⊢ M : A ® m ∈ sigma_glu_exp_pred i FR FP FEl elem_rel SEl }} }.
 
 Variant eq_glu_typ_pred i m n
